\documentclass{beamer}
\input{macros}

\title{ECEn 671: Mathematics of Signals and Systems}
\author{Randal W. Beard}
\institute{Brigham Young University}
\date{\today}

\begin{document}

%-------------------------------
\begin{frame}
	\titlepage
\end{frame}




%%%%%%%%%%%%%%%%%%%%%%%%%%%%%%%%%%%%%%%%%%%%%%%%%%%%%%%%%%%%%%%%%%%%%%%
\section{Gram Schmidt Orthogonalization}
\frame{\sectionpage}


%----------------------------------
\begin{frame}\frametitle{Application:  Gram Schmidt Orthogonalization}
\noindent Given a set $T = \{ p_1, \ldots, p_n\}$

\noindent Find a set $T' = \{q_1, \ldots, q_n'\} \qquad n' \leq n$ such that
\[ span(T') = span(T) \text{ and } <q_i,q_j> = \delta_{ij} \]

\begin{description}
\item[Step 1.]
Normalize the First Vector
\[ q_1 = \frac{p_1}{\norm{ p_1 }} \qquad \text{ (i.e. } \iprod{ q_1,q_1 }=1 \text{ ) } \]
\end{description}
\end{frame}

%----------------------------------
\begin{frame}\frametitle{Application:  Gram Schmidt Orthogonalization, cont}

\begin{description}
\item[Step 2.]	
Let $e_2$ be $p_2$ minus the projection of $p_2$ on $q_1$
i.e.
\[ e_2 = p_2 - \iprod{ p_2, q_1} q_1 \]

\begin{center}
\includegraphics[width=4in]{figures/chap2_gram_schmidt}
\end{center}

Then normalize $e_2$:
\[ q_2 = \frac{e_2}{\norm{ e_2 }} \]
\end{description}
\end{frame}

%----------------------------------
\begin{frame}\frametitle{Application:  Gram Schmidt Orthogonalization, cont}

\begin{description}
\item[Step 3.]
Let $e_k$ be $p_k$ minus the projection of $p_k$ on $q_1, \ldots, q_{k-1}$:
\[ e_k = p_k - \sum_{j=1}^{k-1}\iprod{ p_k, q_j} q_j \Rightarrow q_k = \frac{e_k}{\norm{ e_k }} \]
\end{description}
\end{frame}

%----------------------------------
\begin{frame}\frametitle{Example: Gram Schmidt Orthogonalization}
Given the set
\[
T = \{ p_1, p_2, p_3 \} \defeq \left\{ \begin{pmatrix} 2 \\ 0 \\ 0 \end{pmatrix}, \begin{pmatrix}1 \\ 2 \\ 0 \end{pmatrix}, \begin{pmatrix} 1 \\ 2 \\ 3 \end{pmatrix} \right\}
\]	
find a set $T'=\{q_1, q_2, q_3\}$ where the vectors in $T'$ are orthonormal and $\text{span}(T)=\text{span}(T')$.

\vfill

\[
q_1 = \frac{p_1}{\norm{p_2}} = \frac{\begin{pmatrix} 2 \\ 0 \\ 0 \end{pmatrix}}{2} = \begin{pmatrix} 1 \\ 0 \\ 0 \end{pmatrix}.
\]

\end{frame}

%----------------------------------
\begin{frame}\frametitle{Example: Gram Schmidt Orthogonalization, cont.}

\begin{align*}
e_2 &= p_2 - \iprod{p_2, q_1} q_1 \\
    &= \begin{pmatrix} 1 \\ 2 \\ 0 \end{pmatrix} - \begin{pmatrix} 1\\2\\0\end{pmatrix}^\top\begin{pmatrix}1\\0\\0\end{pmatrix}\begin{pmatrix}1\\0\\0\end{pmatrix} \\
    &= \begin{pmatrix} 1 \\ 2 \\ 0 \end{pmatrix} - 1\cdot\begin{pmatrix}1\\0\\0\end{pmatrix} \\
    &= \begin{pmatrix}0\\2\\0\end{pmatrix}
\end{align*}
Therefore
\(
q_2 = \frac{e_2}{\norm{e_2}} = \frac{\begin{pmatrix}0\\2\\0\end{pmatrix}}{2} = \begin{pmatrix}0\\1\\0\end{pmatrix}
\)

\end{frame}

%----------------------------------
\begin{frame}\frametitle{Example: Gram Schmidt Orthogonalization, cont.}

\begin{align*}
e_3 &= p_3 - \iprod{p_3, q_1} q_1 -\iprod{p_3, q_2}q_2 \\
    &= \begin{pmatrix} 1 \\ 2 \\ 3 \end{pmatrix} - \begin{pmatrix} 1\\2\\3\end{pmatrix}^\top\begin{pmatrix}1\\0\\0\end{pmatrix}\begin{pmatrix}1\\0\\0\end{pmatrix} - \begin{pmatrix} 1\\2\\3\end{pmatrix}^\top\begin{pmatrix}0\\1\\0\end{pmatrix}\begin{pmatrix}0\\1\\0\end{pmatrix} \\
    &= \begin{pmatrix} 1 \\ 2 \\ 3 \end{pmatrix} - 1\cdot\begin{pmatrix}1\\0\\0\end{pmatrix}  - 2\cdot\begin{pmatrix}0\\1\\0\end{pmatrix} \\
    &= \begin{pmatrix}0\\0\\3\end{pmatrix}
\end{align*}
Therefore
\(
q_3 = \frac{e_3}{\norm{e_3}} = \frac{\begin{pmatrix}0\\0\\3\end{pmatrix}}{3} = \begin{pmatrix}0\\0\\1\end{pmatrix}
\)

\end{frame}

%----------------------------------
\begin{frame}\frametitle{Example: Gram Schmidt Orthogonalization, cont.}

Therefore, the Gram Schmidt orthonormalization of 
\[
T = \{ p_1, p_2, p_3 \} \defeq \left\{ \begin{pmatrix} 2 \\ 0 \\ 0 \end{pmatrix}, \begin{pmatrix}1 \\ 2 \\ 0 \end{pmatrix}, \begin{pmatrix} 1 \\ 2 \\ 3 \end{pmatrix} \right\}
\]	
is
\[
T' = \{q_1, q_2, q_3\} = \left\{ \begin{pmatrix} 1 \\ 0 \\ 0 \end{pmatrix}, \begin{pmatrix}0 \\ 1 \\ 0 \end{pmatrix}, \begin{pmatrix} 0 \\ 0 \\ 1 \end{pmatrix} \right\}.
\]

\vfill

Note that $\text{span}(T)=\text{span}(T')$.

\end{frame}




\end{document}