\documentclass{beamer}
\input{macros}

\title{ECEn 671: Mathematics of Signals and Systems}
\author{Randal W. Beard}
\institute{Brigham Young University}
\date{\today}

\begin{document}

%-------------------------------
\begin{frame}
	\titlepage
\end{frame}


%%%%%%%%%%%%%%%%%%%%%%%%%%%%%%%%%%%%%%%%%%%%%%%%%%%%%%%%%%%%%%%%%%
\section{Generalized Fourier Series}
\frame{\sectionpage}

%----------------------------------
\begin{frame}\frametitle{Section 3.17: Generalized Fourier Series}

	Topic of interest: $L_2$ function approximation
	
	\vfill

	\begin{definition}[Complete Basis]
	An orthonormal set $\{p_i, i=1, \ldots, \infty\}$ in a Hilbert space
	$\mathbb{S}$ is a \underline{complete basis} or \underline{total basis} if
	$\forall x \in \mathbb{S}$
	\[ x = \sum_{i=1}^{\infty} \iprod{x,p_i }p_i \]
	\end{definition}
	
	\vfill

	Note that if $x = \sum_{i=1}^{\infty} c_ip_i$ and $\iprod{p_i,p_j } =
	\delta_{ij}$ then
	\[ \iprod{x,p_j } = \sum_{i=1}^{\infty}c_i\iprod{p_i,p_j }=c_j\]
	\[ \Rightarrow c_j = \iprod{x,p_j } \]

	
\end{frame}

%----------------------------------
\begin{frame}\frametitle{Generalized Fourier Series, cont.}
	Therefore we can write
	\[ 
	x = \sum_{i=1}^{\infty} \iprod{x,p_i }p_i.
	\]	
	
	\vfill
	
	Most common example:  standard Fourier basis
	\[ P_n(t) = \frac{1}{\sqrt{T}}e^{j \left(\frac{2\pi}{T}\right)n t} \]
	Any function $f \in L_2[0,T]$ can be written as
	\[ f(t) = \sum_{n=-\infty}^{\infty}c_n \frac{1}{T}
	e^{j\left(\frac{2\pi}{T}\right)nt} \]
	where the coefficients are given as
	\[ c_n = \iprod{f,\frac{1}{\sqrt{T}}e^{j\left(\frac{2\pi}{T}\right)nt} } \defeq
	\frac{1}{\sqrt{T}}\int_{0}^{T}f(t)e^{j\left(\frac{2\pi}{T}\right)nt}dt \]

\end{frame}

%----------------------------------
\begin{frame}\frametitle{Generalized Fourier Series, cont.}
	Actually it is common to place the $\frac{1}{\sqrt{T}}$'s together
	letting $f(t) = \sum_{n=-\infty}^{\infty} b_n e^{j\left(\frac{2\pi}{T}\right)nt}$ where
	\[ b_n = \iprod{f(t), \frac{1}{T}e^{j\left(\frac{2\pi}{T}\right)nt} } =
	\frac{1}{T}\int_0^{T}f(t) e^{-j\left(\frac{2\pi}{T}\right)nt}dt \]
	
	Generalized Fourier series hold for \underline{any} complete basis,
	i.e.
	\[ x = \sum_{j=1}^{\infty} \iprod{x,p_j }p_j \]
	
\end{frame}

%----------------------------------
\begin{frame}\frametitle{Generalized Fourier Series, cont.}
	There are two important relationship between a function and its
	Fourier transform.
	
	\begin{theorem}[Bessel's Inequality]
	Suppose $\{p_1,p_2,\ldots\}$ is orthonormal but not necessarily
	complete and let 
	\[ c = \{ \iprod{x,p_1 },\iprod{x,p_2 }, \ldots \} = \{c_1,c_2,\ldots
	\}\]
	then
	\[ \fbox{$\norm{c }_{\ellbf_2} \leq \norm{x }_{L_2}$} \]
	\end{theorem}

\end{frame}

%----------------------------------
\begin{frame}\frametitle{Proof:}

	\begin{align*}
	0 \leq \norm{x - \sum c_jp_j }_{L_2}^2 &= \iprod{x - \sum c_jp_j, x-
		\sum c_j p_j }_{L_2}\\
	&= \iprod{x,x }_{L_2} 
		- \sum \bar{c}_j\iprod{x,p_j }_{L_2}
	\\ \qquad & 
		- \sum c_j\bar{\iprod{x,p_j }}_{L_2} 
		+ \sum \sum c_j \bar{c}_k \iprod{p_j,p_k
	}_{L_2}\\
	&= \norm{x }_{L_2}^{2} - \sum \bar{c}_jc_j - \sum c_j\bar{c}_j + \sum
	c_j\bar{c}_j\\
	&= \norm{x }_{L_2}^2 - \sum_{j=1}^{\infty} |c_j|^2\\
	&=\norm{x }_{L_2}^2 - \norm{c }_{\ellbf_2}^2\\
	&\Rightarrow \norm{c }_{\ellbf_2}^2 \leq \norm{x }_{L_2}^2
	\end{align*}
\end{frame}

%----------------------------------
\begin{frame}\frametitle{Generalized Fourier Series, cont.}
	\begin{theorem}[Parseval's Equality]
	If $T = \{p_1,p_2,\ldots \}$ is complete then
	\[ \fbox{$\norm{x }_{L_2}^2 = \norm{c }_{\ellbf_2}^2$} \]
	\end{theorem}
	\begin{proof}
	If $T$ is complete then
	\[ \norm{x - \sum c_jp_j }^2 = 0 \]
	and the result follows from the proof of Bessel's inequality	.
	\end{proof}
\end{frame}

%----------------------------------
\begin{frame}\frametitle{Significance of Parseval's Equality}
	
	$\norm{x }_{L_2}^2 = \norm{c }_{\ellbf_2}^2$ says that the energy in a
	signal (i.e. $\norm{x }_{L_2}$) is equal to the energy in the
	Fourier coefficients (i.e. $\norm{c }_{\ellbf_2}^2$).
	
	\vfill
	
	This relationship between $x$ and its transform $c$ is written as 
	\[
	x \overset{\mathcal{F}}{\longleftrightarrow} c.
	\]
	
\end{frame}

%----------------------------------
\begin{frame}\frametitle{Significance of Parseval's Equality, cont.}
	\begin{lemma}[Moon Lemma 3.1]
	If $x \overset{\mathcal{F}}{\longleftrightarrow} c$ and $y \overset{\mathcal{F}}{\longleftrightarrow}
	b$ for the same complete basis $\{p_1,p_2,\ldots\}$ then
	\[ 
	\iprod{x,y }_{L_2} = \iprod{c,b }_{\ellbf_2}.
	\]		
	\end{lemma}
	\begin{proof}
	Let $x = \sum_{i=1}^{\infty} c_ip_i$, and  $y = \sum_{i=1}^{\infty}b_ip_i$
	then
	\begin{align*}
	\iprod{x,y }_{L_2} &=
	\sum_{i=1}^{\infty}\sum_{j=1}^{\infty}c_i\bar{b}_j\iprod{p_i,p_j }\\
	&= \sum_{i=1}^{\infty} c_i\bar{b}_i\\
	&= \iprod{c,b }_{\ellbf_2}
	\end{align*}		
	\end{proof}
\end{frame}




\end{document}